steel/Zeta.Steel.VerifierTypes.fst
@@ -36,7 +36,7 @@ type thread_state_t = {
   thread_id    : tid;
   failed       : R.ref bool;
   store        : vstore;
-  clock        : R.ref U64.t;
+  clock        : R.ref T.timestamp;
   epoch_hashes : AEH.all_epoch_hashes;
   last_verified_epoch: R.ref (option M.epoch_id);
   processed_entries: G.ref (Seq.seq log_entry);
